No more PEnvironment
Precision defined using two LIR environments and explicit proofs
of their precision when needed. (Seems much simpler.)

precision.v
@@ -113,6 +113,17 @@ Proof.
 Qed.
 
 
+(* Nothing is smaller than the empty environment *)
+Lemma EnvCompEmpty : forall Γ, Γ <E| MEmpty -> Γ = MEmpty.
+Proof.
+  destruct Γ; trivial.
+  intros H.
+  specialize (H s).
+  erewrite InEq in H.
+  inversion H.
+Qed.
+
+
 (*
 ** Environment precision is transitive
 *)
@@ -137,8 +148,10 @@ Qed.
 (*
 ** Extending environments preserve precision
 *)
-Lemma EnvCompExt : forall Γ1 Γ2 var t,
-    Γ1 <E| Γ2 -> (var |=> t; Γ1) <E| (var |=> t; Γ2).
+Lemma EnvCompExt : forall Γ1 Γ2 var t1 t2,
+    Γ1 <E| Γ2 ->
+    t1 <| t2 ->
+    (var |=> t1; Γ1) <E| (var |=> t2; Γ2).
 Proof.
   unfold EnvComp.
   intros.
@@ -148,195 +161,19 @@ Proof.
 Qed.
 
 
-(*
-** Environments for precision of expressions:
-** Pairs of environments)
-*)
-Inductive PEnvironment :=
-| PEnv : forall Γ1 Γ2, Γ1 <E| Γ2 -> PEnvironment.
-
-
-(*
-** Empty environment for precision
-*)
-Definition PEmpty : PEnvironment.
-refine (PEnv MEmpty MEmpty _).
-  unfold EnvComp.
-  intros. simpl. constructor.
-Defined.
-
-
-(*
-** Projection 1
-*)
-Definition PEnv1 (Γ : PEnvironment) : IREnvironment :=
-  match Γ with
-  | PEnv Γ1 _ _ => Γ1
-  end.
-
-
-(*
-** Projection 2
-*)
-Definition PEnv2 (Γ : PEnvironment) : IREnvironment :=
-  match Γ with
-  | PEnv _ Γ2 _ => Γ2
-  end.
-
-
-Lemma PEnvIn : forall Γ var t1 t2,
-    In (PEnv1 Γ) var = Some t1 ->
-    In (PEnv2 Γ) var = Some t2 ->
+Lemma PEnvIn : forall Γ1 Γ2 var t1 t2,
+    Γ1 <E| Γ2 ->
+    In Γ1 var = Some t1 ->
+    In Γ2 var = Some t2 ->
     t1 <| t2.
 Proof.
-  intros Γ var t1 t2 H1 H2.
-  destruct Γ.
-  unfold EnvComp in e.
-  simpl in *.
-  specialize (e var).
-  rewrite H1 in e.
-  rewrite H2 in e.
-  inversion e. trivial.
+  intros * HP H1 H2.
+  specialize (HP var).
+  rewrite H1 in HP.
+  rewrite H2 in HP.
+  inversion HP. trivial.
 Qed.
 
-
-(*
-** Create a precision environment with two copies
-** of a given environment
-*)
-Definition Env2P : IREnvironment -> PEnvironment.
-refine (fun Γ => (PEnv Γ Γ _)).
-  unfold EnvComp. intros var.
-  destruct (In Γ var); auto using TPrecOption, TPrecisionRefl.
-Defined.
-
-
-Definition ExpandPEnv : PEnvironment -> string ->
-    forall t1 t2, t1 <| t2 -> PEnvironment.
-refine (fun Γ var t1 t2 H12 =>
-    match Γ with
-    | PEnv Γ1 Γ2 H12' => PEnv (var |=> t1; Γ1) (var |=> t2; Γ2) _
-    end).
-  unfold EnvComp; intros var'.
-  simpl.
-  destruct (string_dec var' var); auto using TPrecOption.
-Defined.
-
-
-(*
-** How 'ExpandPEnv' affects the first environment
-*)
-Lemma Expand1 : forall Γ var t1 t2 H12,
-    PEnv1 (ExpandPEnv Γ var t1 t2 H12) = (var |=> t1; PEnv1 Γ).
-Proof. intros Γ. destruct Γ. trivial. Qed.
-
-
-(*
-** How 'ExpandPEnv' affects the second environment
-*)
-Lemma Expand2 : forall Γ var t1 t2 H12,
-    PEnv2 (ExpandPEnv Γ var t1 t2 H12) = (var |=> t2; PEnv2 Γ).
-Proof. intros Γ. destruct Γ. trivial. Qed.
-
-
-Lemma Env2Env : forall Γ, PEnv1 (Env2P Γ) = Γ.
-Proof. intros Γ. trivial. Qed.
-
-
-(*
-** Two PEnv are equivalent if their environments are equivalent
-*)
-Definition PEquiv (Γ Γ' : PEnvironment) : Prop :=
-  (forall var, In (PEnv1 Γ) var = In (PEnv1 Γ') var) /\
-  (forall var, In (PEnv2 Γ) var = In (PEnv2 Γ') var).
-
-
-(*
-** PEquiv is an equivalence relation
-*)
-
-Lemma PEquivRefl : forall Γ, PEquiv Γ Γ.
-Proof.
-  unfold PEquiv.
-  intros Γ.
-  intuition trivial.
-Qed.
-
-Lemma PEquivSym : forall Γ1 Γ2, PEquiv Γ1 Γ2 -> PEquiv Γ2 Γ1.
-Proof.
-  unfold PEquiv.
-  intros Γ1 Γ2 H.
-  intuition congruence.
-Qed.
-
-Lemma PEquivTrans : forall Γ1 Γ2 Γ3,
-    PEquiv Γ1 Γ2 -> PEquiv Γ2 Γ3 -> PEquiv Γ1 Γ3.
-Proof.
-  unfold PEquiv.
-  intros Γ1 Γ2 Γ3 H12 H23.
-  intuition congruence.
-Qed.
-
-
-(*
-** Shadowing a variable gives a result that is equivalent to
-** one without the shadowed entry
-*)
-Lemma PEquivShadow : forall Γ var t0 t1 t2 t3 H12 H12' H03,
-  PEquiv (ExpandPEnv Γ var t1 t2 H12)
-         (ExpandPEnv (ExpandPEnv Γ var t0 t3 H03) var t1 t2 H12').
-Proof.
-  unfold PEquiv.
-  intros *.
-  destruct Γ. simpl.
-  split; intros; breakStrDec.
-Qed.
-
-(*
-** Changind the order of addition of two different variables gives
-** equivalent results
-*)
-Lemma PEquivPermute : forall Γ var var' t1 t2 t1' t2' H12 H12' H12'' H12''',
-  var <> var' ->
-  PEquiv (ExpandPEnv (ExpandPEnv Γ var t1 t2 H12) var' t1' t2' H12')
-         (ExpandPEnv (ExpandPEnv Γ var' t1' t2' H12'') var t1 t2 H12''').
-Proof.
-  unfold PEquiv.
-  intros *.
-  destruct Γ. simpl.
-  split; intros; breakStrDec.
-Qed.
-
-
-(*
-** Expanding environments with the same element preserves
-** equivalence.
-*)
-Lemma ExpandEquiv : forall Γ1 Γ2 var t1 t2 P1 P2,
-    PEquiv Γ1 Γ2 ->
-    PEquiv (ExpandPEnv Γ1 var t1 t2 P1) (ExpandPEnv Γ2 var t1 t2 P2).
-Proof.
-  unfold PEquiv.
-  intros * HPE.
-  repeat rewrite Expand1 in *.
-  repeat rewrite Expand2 in *.
-  simpl.
-  split; intros; breakStrDec.
-Qed.
-
-
-(*
-** Expanding and duplicating commute (up to equivalence)
-*)
-Lemma Expand2P : forall Γ var t,
-    PEquiv (Env2P (var |=> t; Γ))
-            (ExpandPEnv (Env2P Γ) var t t (TPrecisionRefl t)).
-Proof.
-  intros Γ var t.
-  unfold PEquiv.
-  simpl.
-  split; intros; breakStrDec.
-Qed.
 
 
 (*
@@ -344,91 +181,96 @@ Qed.
 *)
 
 (*
-** (Precision Γ e1 τ1 e2 τ2) means Γ⊑ ⊢ e1 ⊑ e2 : τ1 ⊑ τ2.
-** In words: In the precision environment Γ,
-** the expression e1 with type τ1 is more (or equally) precise
-** than the expression e2 with type τ2.
+** (Precision Γ e1 τ1 Δ e2 τ2) means Γ⊑Δ ⊢ e1 ⊑ e2 : τ1 ⊑ τ2.
+** In words: the expression e1 with type τ1 in the environment Γ is
+** more (or equally) precise than the expression e2 with type τ2 in the
+** environment Δ.
 *)
-Inductive Precision : PEnvironment -> IRE -> IRType ->
-                                      IRE -> IRType -> Prop :=
+Inductive Precision : IREnvironment -> IRE -> IRType ->
+                      IREnvironment -> IRE -> IRType -> Prop :=
 
-(* ----------------------
+(*  Γ ⊑ Δ
+   ----------------------
    Γ⊑ ⊢ nil ⊑ nil : nil ⊑ nil       *)
-| PNil : forall Γ, Precision Γ IRENil IRTNil IRENil IRTNil
+| PNil : forall Γ Δ, Γ <E| Δ -> Precision Γ IRENil IRTNil Δ IRENil IRTNil
 
-(* Γ⊑ ∋ (x : σ ⊑ τ)
-------------------
-Γ⊑ ⊢ x ⊑ x : σ ⊑ τ	*)
-| PVar : forall Γ var t1 t2,
-    In (PEnv1 Γ) var = Some t1 ->
-    In (PEnv2 Γ) var = Some t2 ->
-    Precision Γ (IREVar var) t1 (IREVar var) t2
 
-(* ----------------------
+(* Γ ⊑ Δ    (x : σ) ∈ Γ   (x : τ) ∈ Δ
+  -----------------------------------
+  Γ ⊢ x : σ ⊑ Δ ⊢ x : τ	*)
+| PVar : forall Γ Δ var t1 t2,
+    Γ <E| Δ ->
+    In Γ var = Some t1 ->
+    In Δ var = Some t2 ->
+    Precision Γ (IREVar var) t1 Δ (IREVar var) t2
+
+(* Γ ⊑ Δ
+   ----------------------
    Γ⊑ ⊢ n ⊑ n : int ⊑ int	*)
-| PNum : forall Γ n, Precision Γ (IRENum n) IRTInt (IRENum n) IRTInt
+| PNum : forall Γ Δ n, Γ <E| Δ -> Precision Γ (IRENum n) IRTInt Δ (IRENum n) IRTInt
 
 (* Γ⊑ ⊢ d₁ ⊑ e₁ : int ⊑ int   Γ⊑ ⊢ d₂ ⊑ e₂ : int ⊑ int
    ----------------------------------------------------
    Γ⊑ ⊢ d₁ + d₂ ⊑ e₁ + e₂ : int ⊑ int	*)
-| PPlus : forall Γ d1 e1 d2 e2,
-    Precision Γ d1 IRTInt e1 IRTInt ->
-    Precision Γ d2 IRTInt e2 IRTInt ->
-    Precision Γ (IREPlus d1 d2) IRTInt (IREPlus e1 e2) IRTInt
+| PPlus : forall Γ Δ d1 e1 d2 e2,
+    Precision Γ d1 IRTInt Δ e1 IRTInt ->
+    Precision Γ d2 IRTInt Δ e2 IRTInt ->
+    Precision Γ (IREPlus d1 d2) IRTInt Δ (IREPlus e1 e2) IRTInt
 
-(* ----------------------
+(* Γ ⊑ Δ
+   ----------------------
    Γ⊑ ⊢ {} ⊑ {} : tbl ⊑ tbl	*)
-| PNew : forall Γ, Precision Γ IRENew IRTTbl IRENew IRTTbl
+| PNew : forall Γ Δ, Γ <E| Δ -> Precision Γ IRENew IRTTbl Δ IRENew IRTTbl
 
-(* ----------------------
+(* Γ ⊑ Δ
+   ----------------------
    Γ⊑ ⊢ a ⊑ a : tbl ⊑ tbl	*)
-| PTAddr : forall Γ addr, Precision Γ (IRETAddr addr) IRTTbl
-                                      (IRETAddr addr) IRTTbl
+| PTAddr : forall Γ Δ addr, Γ <E| Δ -> Precision Γ (IRETAddr addr) IRTTbl
+                                                 Δ (IRETAddr addr) IRTTbl
 
 (* ----------------------
    Γ⊑ ⊢ a ⊑ a : fun ⊑ fun	*)
-| PFAddr : forall Γ addr, Precision Γ (IREFAddr addr) IRTFun
-                                      (IREFAddr addr) IRTFun
+| PFAddr : forall Γ Δ addr, Γ <E| Δ -> Precision Γ (IREFAddr addr) IRTFun
+                                                 Δ (IREFAddr addr) IRTFun
 
 
 (* Γ⊑ ⊢ d₁ ⊑ e₁ : tbl ⊑ tbl   Γ⊑ ⊢ d₂ ⊑ e₂ : * ⊑ *
    ----------------------------------------------------
    Γ⊑ ⊢ d₁[d₂] ⊑ e₁[e₂] : * ⊑ *	*)
-| PGet : forall Γ d1 d2 i1 i2,
-    Precision Γ d1 IRTTbl d2 IRTTbl ->
-    Precision Γ i1 IRTStar i2 IRTStar ->
-    Precision Γ (IREGet d1 i1) IRTStar (IREGet d2 i2) IRTStar
+| PGet : forall Γ Δ d1 d2 i1 i2,
+    Precision Γ d1 IRTTbl Δ d2 IRTTbl ->
+    Precision Γ i1 IRTStar Δ i2 IRTStar ->
+    Precision Γ (IREGet d1 i1) IRTStar Δ (IREGet d2 i2) IRTStar
 
-| PSet : forall Γ d1 d2 i1 i2 v1 v2,
-    Precision Γ d1 IRTTbl d2 IRTTbl ->
-    Precision Γ i1 IRTStar i2 IRTStar ->
-    Precision Γ v1 IRTStar v2 IRTStar ->
-    Precision Γ (IRESet d1 i1 v1) IRTNil (IRESet d2 i2 v2) IRTNil
+| PSet : forall Γ Δ d1 d2 i1 i2 v1 v2,
+    Precision Γ d1 IRTTbl Δ d2 IRTTbl ->
+    Precision Γ i1 IRTStar Δ i2 IRTStar ->
+    Precision Γ v1 IRTStar Δ v2 IRTStar ->
+    Precision Γ (IRESet d1 i1 v1) IRTNil Δ (IRESet d2 i2 v2) IRTNil
 
 (* Γ⊑, x : σ ⊑ τ ⊢ d₂ ⊑ e₂ : σ′ ⊑ τ′    Γ⊑ ⊢ d₁ ⊑ e₁ : σ ⊑ τ
    -------------------------------------------------------
    Γ⊑ ⊢ let x:σ = d₁ in d₂ ⊑ let x:τ = e₁ in e₂ : σ′ ⊑ τ′	*)
-| PLet : forall Γ var d1 t1 d2 t2 b1 t1' b2 t2' H12,
-    Precision (ExpandPEnv Γ var t1 t2 H12) b1 t1' b2 t2' ->
-    Precision Γ d1 t1 d2 t2 ->
-    Precision Γ (IRELet var t1 d1 b1) t1' (IRELet var t2 d2 b2) t2'
+| PLet : forall Γ Δ var d1 t1 d2 t2 b1 t1' b2 t2',
+    Precision (var |=> t1; Γ) b1 t1' (var |=> t2; Δ) b2 t2' ->
+    Precision Γ d1 t1 Δ d2 t2 ->
+    Precision Γ (IRELet var t1 d1 b1) t1' Δ (IRELet var t2 d2 b2) t2'
 
 (* Γ⊑, x : * ⊑ * ⊢ d ⊑ e : * ⊑ *
    --------------------------------
    Γ⊑ ⊢ (λx.d) ⊑ (λx.e) : fun ⊑ fun	*)
-| PFun : forall Γ var d1 d2,
-    Precision (ExpandPEnv Γ var IRTStar IRTStar (TPrecisionRefl IRTStar))
-                 d1 IRTStar d2 IRTStar ->
-    Precision Γ (IREFun var d1) IRTFun
-                (IREFun var d2) IRTFun
+| PFun : forall Γ Δ var d1 d2,
+    Precision (var |=> IRTStar; Γ) d1 IRTStar (var |=> IRTStar; Δ) d2 IRTStar ->
+    Γ <E| Δ ->
+    Precision Γ (IREFun var d1) IRTFun Δ (IREFun var d2) IRTFun
 
 (* Γ⊑ ⊢ d₁ ⊑ e₁ : fun ⊑ fun    Γ⊑ ⊢ d₂ ⊑ e₂ : * ⊑ *
   -------------------------------------------------
   Γ⊑ ⊢ d₁(d₂) ⊑ e₁(e₂) : * ⊑ *	*)
-| PApp : forall Γ f1 v1 f2 v2,
-    Precision Γ v1 IRTStar v2 IRTStar ->
-    Precision Γ f1 IRTFun f2 IRTFun ->
-    Precision Γ (IREApp f1 v1) IRTStar (IREApp f2 v2) IRTStar
+| PApp : forall Γ Δ f1 v1 f2 v2,
+    Precision Γ v1 IRTStar Δ v2 IRTStar ->
+    Precision Γ f1 IRTFun Δ f2 IRTFun ->
+    Precision Γ (IREApp f1 v1) IRTStar Δ (IREApp f2 v2) IRTStar
 
 (* Γ⊑ ⊢ d ⊑ e : t ⊑ g
    ----------------------------------
@@ -436,33 +278,33 @@ Inductive Precision : PEnvironment -> IRE -> IRType ->
 (* Note: in our particular case, t must be equal to g, because
    g is a ground type and there is no type strictly more precise
    than a ground type. *)
-| PBoxR : forall Γ d e t g,
-    Precision Γ d t e (Tag2Type g) ->
-    Precision Γ d t (IREBox g e) IRTStar
+| PBoxR : forall Γ Δ d e t g,
+    Precision Γ d t Δ e (Tag2Type g) ->
+    Precision Γ d t Δ (IREBox g e) IRTStar
 
 (* Γ⊑ ⊢ d ⊑ e : g ⊑ ★
    ----------------------------------
    Γ⊑ ⊢ box[g]d ⊑ e : ★ ⊑ ★	*)
-| PBoxL : forall Γ d e g,
-    Precision Γ d (Tag2Type g) e IRTStar ->
-    Precision Γ (IREBox g d) IRTStar e IRTStar
+| PBoxL : forall Γ Δ d e g,
+    Precision Γ d (Tag2Type g) Δ e IRTStar ->
+    Precision Γ (IREBox g d) IRTStar Δ e IRTStar
 
 (* Γ⊑ ⊢ d ⊑ e : ★ ⊑ ★
    ----------------------------------
    Γ⊑ ⊢ unbox[g](d) ⊑ e : g ⊑ *		*)
-| PUnboxL : forall Γ d e g tg,
+| PUnboxL : forall Γ Δ d e g tg,
     tg = Tag2Type g ->
-    Precision Γ d IRTStar e IRTStar ->
-    Precision Γ (IREUnbox g d) tg e IRTStar
+    Precision Γ d IRTStar Δ e IRTStar ->
+    Precision Γ (IREUnbox g d) tg Δ e IRTStar
 
 (* Γ⊑ ⊢ d ⊑ e : t ⊑ ★ , t ⊑ g
    ----------------------------------
    Γ⊑ ⊢ d ⊑ unbox[g](e) : t ⊑ g	*)
-| PUnboxR : forall Γ d e t g tg,
+| PUnboxR : forall Γ Δ d e t g tg,
     t <| (Tag2Type g) ->
     tg = Tag2Type g ->
-    Precision Γ d t e IRTStar ->
-    Precision Γ d t (IREUnbox g e) tg
+    Precision Γ d t Δ e IRTStar ->
+    Precision Γ d t Δ (IREUnbox g e) tg
 
 .
 
@@ -470,18 +312,18 @@ Inductive Precision : PEnvironment -> IRE -> IRType ->
 (* Γ⊑ ⊢ d ⊑ e : g ⊑ g
    ----------------------------------
    Γ⊑ ⊢ box[g](d) ⊑ box[g](e) : ★ ⊑ ★	*)
-Lemma BoxCongruent : forall Γ d e g,
-    Precision Γ d (Tag2Type g) e (Tag2Type g) ->
-    Precision Γ (IREBox g d) IRTStar (IREBox g e) IRTStar.
+Lemma BoxCongruent : forall Γ Δ d e g,
+    Precision Γ d (Tag2Type g) Δ e (Tag2Type g) ->
+    Precision Γ (IREBox g d) IRTStar Δ (IREBox g e) IRTStar.
 Proof. eauto using Precision. Qed.
 
 
 (* Γ⊑ ⊢ d ⊑ e : ★ ⊑ ★
    ----------------------------------
    Γ⊑ ⊢ unbox[g](d) ⊑ unbox[g](e) : g ⊑ g	*)
-Lemma UnboxCongruent: forall Γ d e g,
-    Precision Γ d IRTStar e IRTStar ->
-    Precision Γ (IREUnbox g d) (Tag2Type g) (IREUnbox g e) (Tag2Type g).
+Lemma UnboxCongruent: forall Γ Δ d e g,
+    Precision Γ d IRTStar Δ e IRTStar ->
+    Precision Γ (IREUnbox g d) (Tag2Type g) Δ (IREUnbox g e) (Tag2Type g).
 Proof. eauto using Precision, TPrecisionRefl. Qed.
 
 
@@ -525,8 +367,8 @@ Qed.
 
 
 (* Expressions related by Precision differ only in boxes and unboxes *)
-Lemma EqBones : forall Γ e1 t1 e2 t2,
-  Precision Γ e1 t1 e2 t2 -> Tbones e1 = Tbones e2.
+Lemma EqBones : forall Γ Δ e1 t1 e2 t2,
+  Precision Γ e1 t1 Δ e2 t2 -> Tbones e1 = Tbones e2.
 Proof.
   intros * HP.
   induction HP; trivial; simpl; congruence.
@@ -540,19 +382,19 @@ Definition B10 := (IREBox TgInt (IRENum 10)).
 Definition UB10 := IREUnbox TgInt B10.
 
 (* 10 ⊑ unbox[int](box[int](10)) : int ⊑ int *)
-Example example1 : Precision PEmpty (IRENum 10) IRTInt UB10 IRTInt.
-  eauto using Precision, TPrecisionRefl.
+Example example1 : Precision MEmpty (IRENum 10) IRTInt MEmpty UB10 IRTInt.
+  eauto using Precision, TPrecisionRefl, EnvCompRefl.
 Qed.
 
 (* FALSE!  unbox[int](box[int](10)) ⊑ 10 : int ⊑ int *)
-Example example2 : ~ Precision PEmpty UB10 IRTInt (IRENum 10) IRTInt.
+Example example2 : ~ Precision MEmpty UB10 IRTInt MEmpty (IRENum 10) IRTInt.
   intros HF.
   inversion HF.
 Qed.
 
 (* unbox[int](box[int](10)) ⊑ box[int](10) : int ⊑ * *)
-Example example3 : Precision PEmpty UB10 IRTInt B10 IRTStar.
-  eauto using Precision.
+Example example3 : Precision MEmpty UB10 IRTInt MEmpty B10 IRTStar.
+  eauto using Precision, EnvCompRefl.
 Qed.
 
 (*
@@ -561,25 +403,25 @@ Qed.
 *)
 Definition X := "x":string.
 
-Goal Precision PEmpty
+Goal Precision MEmpty
   (IRELet X IRTInt (IRENum 10)
      (IREPlus (IREVar X) (IRENum 1)))  IRTInt
+    MEmpty
   (IRELet X IRTStar (IREBox TgInt(IRENum 10))
      (IREPlus (IREUnbox TgInt (IREVar X)) (IRENum 1))) IRTInt.
 Proof.
   unfold IRTInt.
   eapply PLet.
-  - eapply PPlus; unfold IRTInt; eauto using Precision, TPrecision.
-  - eauto using Precision.
-  Unshelve. auto using TPrecision.
+  - eapply PPlus; unfold IRTInt;
+    eauto using Precision, TPrecision, EnvCompRefl, EnvCompExt.
+  - eauto using Precision, EnvCompRefl.
 Qed.
-
 
 
 
 (* Nothing is smaller than 10 *)
 Goal forall E T,
-  Precision PEmpty E T (IRENum 10) IRTInt ->
+  Precision MEmpty E T MEmpty (IRENum 10) IRTInt ->
   E = IRENum 10.
 Proof.
   intros * HP.
@@ -590,7 +432,7 @@ Qed.
 (* Precision does not preserve values in any direction *)
 
 Goal exists e1 t1 e2 t2,
-    Precision PEmpty e1 t1 e2 t2 /\ Value e1 /\ ~Value e2.
+    Precision MEmpty e1 t1 MEmpty e2 t2 /\ Value e1 /\ ~Value e2.
   eexists; eexists; eexists; eexists.
   split; try split.
   - apply example1.
@@ -599,7 +441,7 @@ Goal exists e1 t1 e2 t2,
 Qed.
 
 Goal exists e1 t1 e2 t2,
-    Precision PEmpty e1 t1 e2 t2 /\ Value e2 /\ ~Value e1.
+    Precision MEmpty e1 t1 MEmpty e2 t2 /\ Value e2 /\ ~Value e1.
   eexists; eexists; eexists; eexists.
   split; try split.
   - apply example3.
@@ -609,9 +451,9 @@ Qed.
 
 
 (* Types inside precision-related expressions can go astray... *)
-Goal Precision PEmpty (IREBox TgTbl (IREUnbox TgTbl B10)) IRTStar B10 IRTStar.
+Goal Precision MEmpty (IREBox TgTbl (IREUnbox TgTbl B10)) IRTStar MEmpty B10 IRTStar.
 Proof.
-  eauto using Precision.
+  eauto 6 using Precision, EnvCompRefl.
 Qed.
 
 (*
@@ -619,12 +461,12 @@ Qed.
 ** for 10 (everything larger than 10 is smaller than B10), 10 is not
 ** a minimum for B10...
 *)
-Goal ~ Precision PEmpty (IRENum 10) IRTInt
-                        (IREBox TgTbl (IREUnbox TgTbl B10)) IRTStar.
+Goal ~ Precision MEmpty (IRENum 10) IRTInt
+                 MEmpty (IREBox TgTbl (IREUnbox TgTbl B10)) IRTStar.
 Proof.
   intros H.
   inversion H; subst.
-  inversion H4; subst.
+  inversion H5; subst.
   inversion H2.
 Qed.
 
@@ -634,30 +476,30 @@ Definition get10 (a : nat) := IREGet (IRETAddr a) B10.
 
 (* unbox[int](a[10]) ⊑ a[10] *)
 Goal forall a,
-    Precision PEmpty (IREUnbox TgInt (get10 a)) (Tag2Type TgInt)
-                     (get10 a) IRTStar.
+    Precision MEmpty (IREUnbox TgInt (get10 a)) (Tag2Type TgInt)
+              MEmpty (get10 a) IRTStar.
 Proof.
-  eauto using Precision.
+  eauto 7 using Precision, EnvCompRefl.
 Qed.
 
 
 (* box[int](unbox[int](a[10])) ⊑ a[10] *)
-Goal forall a, Precision PEmpty
-    (IREBox TgInt (IREUnbox TgInt (get10 a))) IRTStar
-                     (get10 a) IRTStar.
+Goal forall a, Precision
+                 MEmpty (IREBox TgInt (IREUnbox TgInt (get10 a))) IRTStar
+                 MEmpty (get10 a) IRTStar.
 Proof.
-  eauto 6 using Precision.
+  eauto 8 using Precision, EnvCompRefl.
 Qed.
 
 
 (* ~ a[10] ⊑ box[int](unbox[int](a[10])) *)
-Goal forall a, ~ Precision PEmpty
-    (get10 a) IRTStar
-    (IREBox TgInt (IREUnbox TgInt (get10 a))) IRTStar.
+Goal forall a, ~ Precision
+                   MEmpty (get10 a) IRTStar
+                   MEmpty (IREBox TgInt (IREUnbox TgInt (get10 a))) IRTStar.
 Proof.
   intros * H.
   inversion H; subst.
-  inversion H4; subst.
+  inversion H5; subst.
   inversion H2.
 Qed.
 
@@ -669,96 +511,38 @@ Qed.
 Definition BUB10 := IREBox TgInt UB10.
 
 (* box[int](unbox[int](box[int](10))) ⊑ box[int](10) : * ⊑ * *)
-Example e6 : Precision PEmpty BUB10 IRTStar B10 IRTStar.
-  eauto using Precision.
+Example e6 : Precision MEmpty BUB10 IRTStar MEmpty B10 IRTStar.
+  eauto 6 using Precision, EnvCompRefl.
 Qed.
 
 (* box[int](10) ⊑ box[int](unbox[int](box[int](10))) : * ⊑ * *)
-Example e7 : Precision PEmpty B10 IRTStar BUB10 IRTStar.
-  eauto using Precision, TPrecisionRefl.
+Example e7 : Precision MEmpty B10 IRTStar MEmpty BUB10 IRTStar.
+  eauto 6 using Precision, TPrecisionRefl, EnvCompRefl.
 Qed.
 
 End Examples.
 
 
-(* Inclusion for precision environments *)
-Definition Pinclusion (Γ Γ' : PEnvironment) : Prop :=
-  inclusion (PEnv1 Γ) (PEnv1 Γ') /\ inclusion (PEnv2 Γ) (PEnv2 Γ').
-
-
-Lemma PinclusionEmpty : forall Γ, Pinclusion PEmpty Γ.
-Proof.
-  intros.
-  unfold Pinclusion. simpl.
-  auto using inclusion_empty.
-Qed.
-
 
 (* For precision environments, equivalence implies inclusion *)
-Lemma PinclusionEquiv : forall Γ Γ',
-    PEquiv Γ Γ' -> Pinclusion Γ Γ'.
+Lemma PinclusionEquiv : forall (Γ Γ' : IREnvironment),
+    map_eq Γ Γ' -> inclusion Γ Γ'.
 Proof.
   intros * H.
-  destruct H.
-  unfold Pinclusion.
   intuition congruence.
 Qed.
 
 
-(* Expansion preserves inclusion *)
-Lemma PinclusionExpand : forall Γ Γ' var t1 t2 H12,
-    Pinclusion Γ Γ' ->
-    Pinclusion (ExpandPEnv Γ var t1 t2 H12)
-               (ExpandPEnv Γ' var t1 t2 H12).
-Proof.
-  unfold Pinclusion.
-  intros * HIn.
-  destruct Γ. destruct Γ'.
-  simpl in *. destruct HIn.
-  auto using inclusion_update.
-Qed.
-
-
-Lemma ExpandShadow : forall Γ var t0 t1 t2 t3 H12 H12',
-    Pinclusion
-      (ExpandPEnv (ExpandPEnv Γ var t1 t2 H12) var t0 t3 H12')
-      (ExpandPEnv Γ var t0 t3 H12').
-Proof.
-  intros.
-  unfold Pinclusion.
-  destruct Γ.
-  simpl.
-  auto using inclusion_shadow.
-Qed.
-
-
 (*
-** Precision is preserved if we extend PEnv
-** with extra variables
+** The environments in a precision relation must be
+** in a precision relation too.
 *)
-Lemma PrecisionInclusion : forall Γ Γ' e1 t1 e2 t2,
-    Pinclusion Γ Γ' ->
-    Precision Γ e1 t1 e2 t2 ->
-    Precision Γ' e1 t1 e2 t2.
+Lemma PPE : forall Γ Δ e1 t1 e2 t2,
+    Precision Γ e1 t1 Δ e2 t2 -> Γ <E| Δ.
 Proof.
-  intros * HI HP.
-  generalize dependent Γ'.
-  induction HP; intros; subst; eauto using Precision, PinclusionExpand.
-  destruct HI.
-  eauto using Precision.
-Qed.
-
-
-(*
-** Precision is preserved if we replace PEnv
-** with an equivalent one.
-*)
-Lemma PrecisionIrrel : forall Γ1 Γ2 e1 t1 e2 t2,
-   PEquiv Γ1 Γ2 ->
-   Precision Γ1 e1 t1 e2 t2 ->
-   Precision Γ2 e1 t1 e2 t2.
-Proof.
-  eauto using PrecisionInclusion, PinclusionEquiv.
+  intros * HP.
+  induction HP; subst; eauto using TPrecision, TPrecisionRefl,
+    PEnvIn.
 Qed.
 
 
@@ -766,66 +550,72 @@ Qed.
 ** The types in a precision relation must be
 ** in a precision relation too.
 *)
-Lemma PPT : forall Γ e1 t1 e2 t2,
-    Precision Γ e1 t1 e2 t2 -> t1 <| t2.
+Lemma PPT : forall Γ Δ e1 t1 e2 t2,
+    Precision Γ e1 t1 Δ e2 t2 -> t1 <| t2.
 Proof.
-  intros Γ e1 t1 e2 t2 HP.
+  intros * HP.
   induction HP; subst; eauto using TPrecision, TPrecisionRefl,
     PEnvIn.
 Qed.
 
 
-(*
-** Precision subsumes typing for its first expression
-*)
-Lemma PrecisionType1: forall Γ e1 t1 e2 t2,
-  Precision Γ e1 t1 e2 t2 -> (PEnv1 Γ) |= e1 : t1.
+Lemma extend2Types : forall Γ Δ var t1 t1' t2 t2' b1 b2,
+    Precision (var |=> t1; Γ) b1 t1' (var |=> t2; Δ) b2 t2' ->
+    t1 <| t2.
 Proof.
-  intros Γ e1 t1 e2 t2 HP.
-  induction HP; subst; eauto using IRTyping;
-  try match goal with
-    [H: context [PEnv1 (ExpandPEnv _ _ _ _ _)] |- _] =>
-      rewrite Expand1 in H end;
-  eauto using IRTyping.
+  intros * HP.
+  apply PPE in HP.
+  specialize (HP var).
+  rewrite InEq in HP.
+  rewrite InEq in HP.
+  inversion HP.
+  trivial.
 Qed.
 
 
-(*
-** Special case for the empty environment
-*)
-Lemma PrecisionType1Empty: forall e1 t1 e2 t2,
-  Precision PEmpty e1 t1 e2 t2 -> MEmpty |= e1 : t1.
+Lemma PrecisionInclusion : forall Γ1 Γ2 Δ1 Δ2 e1 t1 e2 t2,
+    Precision Γ1 e1 t1 Δ1 e2 t2 ->
+    inclusion Γ1 Γ2 ->
+    inclusion Δ1 Δ2 ->
+    Γ2 <E| Δ2 ->
+    Precision Γ2 e1 t1 Δ2 e2 t2.
 Proof.
-  intros.
-  replace MEmpty with (PEnv1 PEmpty) by trivial.
-  eauto using PrecisionType1.
+  intros * HP.
+  generalize dependent Γ2.
+  generalize dependent Δ2.
+  induction HP; intros * HI1 HI2 HE;
+    eauto 8 using Precision, inclusion_update, EnvCompExt, PPT.
+Qed.
+
+
+Lemma PrecisionInclusionE : forall Γ Δ e1 t1 e2 t2,
+    Precision MEmpty e1 t1 MEmpty e2 t2 ->
+    Γ <E| Δ ->
+    Precision Γ e1 t1 Δ e2 t2.
+Proof.
+  intros; eauto using PrecisionInclusion, inclusion_empty.
+Qed.
+  
+
+(*
+** Precision subsumes typing for its first expression
+*)
+Lemma PrecisionType1: forall Γ Δ e1 t1 e2 t2,
+  Precision Γ e1 t1 Δ e2 t2 -> Γ |= e1 : t1.
+Proof.
+  intros * HP.
+  induction HP; eauto using IRTyping.
 Qed.
 
 
 (*
 ** Precision subsumes typing for its second expression
 *)
-Lemma PrecisionType2: forall Γ e1 t1 e2 t2,
-  Precision Γ e1 t1 e2 t2 -> (PEnv2 Γ) |= e2 : t2.
+Lemma PrecisionType2: forall Γ Δ e1 t1 e2 t2,
+  Precision Γ e1 t1 Δ e2 t2 -> Δ |= e2 : t2.
 Proof.
-  intros Γ e1 t1 e2 t2 HP.
-  induction HP; subst;
-  try match goal with
-    [H: context [PEnv2 (ExpandPEnv _ _ _ _ _)] |- _] =>
-      rewrite Expand2 in H end;
-  eauto using IRTyping.
-Qed.
-
-
-(*
-** Special case for the empty environment
-*)
-Lemma PrecisionType2Empty: forall e1 t1 e2 t2,
-  Precision PEmpty e1 t1 e2 t2 -> MEmpty |= e2 : t2.
-Proof.
-  intros.
-  replace MEmpty with (PEnv2 PEmpty) by trivial.
-  eauto using PrecisionType2.
+  intros * HP.
+  induction HP; eauto using IRTyping.
 Qed.
 
 
@@ -833,55 +623,19 @@ Qed.
 ** Precision is relfexive for well-typed terms
 *)
 Lemma PrecisionRefl: forall Γ e t,
-    Γ |= e : t ->  Precision (Env2P Γ) e t e t.
+    Γ |= e : t ->  Precision Γ e t Γ e t.
 Proof.
   intros * Hty.
-  induction Hty; subst; eauto using Precision, UnboxCongruent, Expand2P,
-      PrecisionIrrel.
+  induction Hty; subst; eauto using Precision, UnboxCongruent, EnvCompRefl.
 Qed.
 
 
-(*
-** Precision subsumes typing
-*)
-Lemma PrecisionType: forall Γ e t,
-    Γ |= e : t  <->  Precision (Env2P Γ) e t e t.
+Lemma PEnvDyn : forall Γ, Γ <E| dynGamma Γ.
 Proof.
-  intros Γ e t.
-  split; intros H.
-  - induction H; eapply PrecisionRefl; eauto using IRTyping.
-  - apply PrecisionType1 in H.
-    rewrite Env2Env in H. trivial.
-Qed.
-
-
-(*
-** Make a precision environment with Γ and (dyn Γ).
-*)
-Definition PEnvDyn (Γ : IREnvironment) : PEnvironment.
-refine (PEnv Γ (dynGamma Γ) _).
   unfold EnvComp. intros.
   destruct (In Γ var) eqn:?.
   - rewrite TP2TGammaIn with (T := i); auto using TPrecOption, TPrecision.
   - rewrite NTP2TGammaIn; auto using TPrecOption.
-Defined.
-
-
-Lemma Env2DynEmpty : PEquiv (PEnvDyn MEmpty) PEmpty.
-Proof. unfold PEquiv. split; trivial. Qed.
-
-
-(*
-** Expansion and 'dyn' commutes for precision environments
-** (up to equivalence)
-*)
-Lemma EquivDyn : forall Γ var t P,
-  PEquiv (PEnvDyn (var |=> t; Γ))
-          (ExpandPEnv (PEnvDyn Γ) var t IRTStar P).
-Proof.
-  intros.
-  unfold PEquiv.
-  split; intros; auto.
 Qed.
 
 
@@ -890,15 +644,10 @@ Qed.
 ** the original
 *)
 Theorem DynLessPrecise : forall Γ e t,
-  Γ |= e : t -> Precision (PEnvDyn Γ) e t (dyn e) IRTStar.
+  Γ |= e : t -> Precision Γ e t (dynGamma Γ) (dyn e) IRTStar.
 Proof.
-  intros Γ e t H.
-  induction H; simpl; eauto using Precision, TPrecision, TP2TGammaIn.
-  - apply PVar; unfold PEnvDyn; simpl; eauto using TP2TGammaIn.
-  - apply PLet with (TPStar t);
-    eauto using PrecisionIrrel, EquivDyn.
-  - apply PBoxR. apply PFun.
-    eauto using PrecisionIrrel, EquivDyn.
+  intros * H.
+  induction H; simpl; eauto using Precision, TPrecision, TP2TGammaIn, PEnvDyn.
 Qed.
 
 
@@ -906,8 +655,8 @@ Qed.
 ** Any pair of expressions in a precision relation are equal
 ** up to type erasure.
 *)
-Theorem PrecDynEqual : forall Γ e1 t1 e2 t2,
-    Precision Γ e1 t1 e2 t2 -> dyn e2 = dyn e1.
+Theorem PrecDynEqual : forall Γ Δ e1 t1 e2 t2,
+    Precision Γ e1 t1 Δ e2 t2 -> dyn e2 = dyn e1.
 Proof.
   intros * HP. induction HP; simpl; congruence.
 Qed.
@@ -919,14 +668,13 @@ Qed.
 *)
 Theorem PrecDynEqualVal : forall e1 t1 e2,
     Value e2 ->
-    Precision PEmpty e1 t1 e2 IRTStar ->
+    Precision MEmpty e1 t1 MEmpty e2 IRTStar ->
     e2 = dyn e1.
 Proof.
   intros.
   replace e2 with (dyn e2). eauto using PrecDynEqual.
-  symmetry. apply ValueStar; trivial.
-  replace MEmpty with (PEnv2 PEmpty) by trivial.
-  eauto using PrecisionType2.
+  symmetry.
+  eauto using PrecisionType2, ValueStar.
 Qed.
 
 
@@ -934,9 +682,9 @@ Qed.
 ** (dyn e1) is larger than any expression larger than e1:
 ** forall e2, e1 ⊑ e2  ->  e2 ⊑ dyn (e1)
 *)
-Theorem DynMoreDyn : forall Γ e1 t1 e2 t2,
-  Precision Γ e1 t1 e2 t2 ->
-  Precision (PEnvDyn (PEnv2 Γ)) e2 t2 (dyn e1) IRTStar.
+Theorem DynMoreDyn : forall Γ Δ e1 t1 e2 t2,
+  Precision Γ e1 t1 Δ e2 t2 ->
+  Precision Δ e2 t2 (dynGamma Δ) (dyn e1) IRTStar.
 Proof.
   intros.
   replace (dyn e1) with (dyn e2) by eauto using PrecDynEqual.
